utp_ap_healthy.thy
@@ -4,11 +4,9 @@ theory utp_ap_healthy
   imports "UTP-Reactive-Angelic-Designs.utp_rad"
 begin
 
-subsection \<open>Healthiness Conditions\<close>
+subsection \<open>The Identity of Angelic Processes\<close>
 
-subsubsection \<open>The identity of angelic processes\<close>
-
-(* Paper Definition 47: II_AP = H1 (ok' \<and> s \<in> ac'). *)
+(* Paper Definition 47: II_AP \<equiv> H1 (ok' \<and> s \<in> ac'). *)
 definition II_AP :: "('t::trace, 'e) reactive_angelic_design" where
 [pred]: "II_AP = H1 (ok\<^sup>> \<and> ades_state_choice)"
 
@@ -26,7 +24,11 @@ lemma RA2_II_AP: "RA2 II_AP = II_AP"
 lemma II_AP_is_RA2 [closure]: "II_AP is RA2"
   by (rule Healthy_intro, rule RA2_II_AP)
 
-subsubsection \<open>RA3AP: Waiting\<close>
+lemma II_AP_is_PBMH_ades [closure]: "II_AP is PBMH_ades"
+  by (simp add: Healthy_def' II_AP_design PBMH_ades_def design_def
+      fun_eq_iff; pred_auto; blast)
+
+subsection \<open>RA3AP: Waiting\<close>
 
 (* Paper Definition 48: RA3AP (P) = II_AP \<triangleleft> s.wait \<triangleright> P. *)
 definition RA3AP :: "('t::trace, 'e) reactive_angelic_design \<Rightarrow> ('t, 'e) reactive_angelic_design" where
@@ -56,6 +58,12 @@ lemma RA3AP_II_AP: "RA3AP II_AP = II_AP"
 
 lemma II_AP_is_RA3AP [closure]: "II_AP is RA3AP"
   by (rule Healthy_intro, rule RA3AP_II_AP)
+
+lemma RA3AP_PBMH_ades_closure [closure]:
+  assumes "P is PBMH_ades"
+  shows "RA3AP P is PBMH_ades"
+  unfolding RA3AP_def
+  by (rule rad_wait_cond_PBMH_ades_closure[OF II_AP_is_PBMH_ades assms])
 
 (* Thesis Theorem T.6.2.7. *)
 lemma RA2_RA3AP_commute: "(RA2 \<circ> RA3AP) P = (RA3AP \<circ> RA2) P"
@@ -120,8 +128,8 @@ lemma RA1_RA3AP_RA3: "(RA1 \<circ> RA3AP) P = (RA1 \<circ> RA3) P"
 
 (* II_AP collapses to ades_state_choice under the design's ok. *)
 lemma RA3AP_design_post:
-  "(Pre \<turnstile> RA3AP Q) =
-   (Pre \<turnstile>
+  "(P \<turnstile> RA3AP Q) =
+   (P \<turnstile>
     (ades_state_choice \<triangleleft> $rad_wait_lens\<^sup>< \<triangleright> Q))"
   by (simp add: RA3AP_def II_AP_def H1_def design_def expr_if_def
       fun_eq_iff; pred_auto)
@@ -130,7 +138,7 @@ lemma RA3AP_true_design:
   "RA3AP (true \<turnstile> Y) = (true \<turnstile> RA3AP Y)"
   by (simp only: RA3AP_design_post RA3AP_design expr_if_idem)
 
-subsubsection \<open>AP\<close>
+subsection \<open>AP\<close>
 
 (* Paper Definition 46: AP = RA3AP \<circ> RA2 \<circ> A \<circ> H1 \<circ> CSPA2. *)
 definition AP ::
@@ -163,13 +171,10 @@ proof -
     by (simp add: H1_H2_eq_design)
 qed
 
-(* Paper Theorem 37 / Thesis Theorem T.6.2.9. *)
-theorem AP_design:
-  "AP P =
-   ((true \<triangleleft> $rad_wait_lens\<^sup>< \<triangleright>
-       (\<not> (RA2 \<circ> PBMH_ades) ((P \<^sub>wf)\<^sup>f))) \<turnstile>
-    (ades_state_choice \<triangleleft> $rad_wait_lens\<^sup>< \<triangleright>
-       (RA2 \<circ> RA1 \<circ> PBMH_ades) ((P \<^sub>wf)\<^sup>t)))"
+(* Paper Theorem 37 / Thesis Theorem T.6.2.9 *)
+theorem AP_wait_cond_design:
+  "AP P = ((true \<triangleleft> $rad_wait_lens\<^sup>< \<triangleright> (\<not> (RA2 \<circ> PBMH_ades) ((P \<^sub>wf)\<^sup>f))) \<turnstile>
+    (ades_state_choice \<triangleleft> $rad_wait_lens\<^sup>< \<triangleright> (RA2 \<circ> RA1 \<circ> PBMH_ades) ((P \<^sub>wf)\<^sup>t)))"
 proof -
   let ?F = "(P \<^sub>wf)\<^sup>f" and ?T = "(P \<^sub>wf)\<^sup>t"
   have "AP P = (RA3AP \<circ> RA2 \<circ> A) ((\<not> ?F) \<turnstile> ?T)"
@@ -190,47 +195,32 @@ qed
 
 (* Theorem 37 with the wait conditionals folded into RA3AP. *)
 lemma AP_RA3AP_design:
-  "AP P =
-   RA3AP ((\<not> (RA2 \<circ> PBMH_ades) ((P \<^sub>wf)\<^sup>f)) \<turnstile>
+  "AP P = RA3AP ((\<not> (RA2 \<circ> PBMH_ades) ((P \<^sub>wf)\<^sup>f)) \<turnstile>
           (RA2 \<circ> RA1 \<circ> PBMH_ades) ((P \<^sub>wf)\<^sup>t))"
-  by (simp only: AP_design RA3AP_design comp_apply)
+  by (simp only: AP_wait_cond_design RA3AP_design comp_apply)
 
 (* Counterpart of RA_true_design. *)
 lemma AP_true_design:
-  assumes "(Post \<^sub>wf) = Post" "PBMH_ades Post = Post"
-    and "Post\<lbrakk>True/ok\<^sup>>\<rbrakk> = Post"
-  shows "AP (true \<turnstile> Post) =
+  assumes "(Q \<^sub>wf) = Q" "PBMH_ades Q = Q"
+    and "Q\<lbrakk>True/ok\<^sup>>\<rbrakk> = Q"
+  shows "AP (true \<turnstile> Q) =
     (true \<turnstile>
      (ades_state_choice \<triangleleft> $rad_wait_lens\<^sup>< \<triangleright>
-      RA1 (RA2 Post)))"
+      RA1 (RA2 Q)))"
 proof -
-  let ?P = "(true \<turnstile> Post)"
-  have wf_id: "(?P \<^sub>wf) = ?P"
-    by (simp only: rad_wait_false_design rad_wait_false_true assms(1))
-  have proj_f: "?P\<^sup>f = (\<not> ok\<^sup><)"
-    by pred_auto
-  have proj_t_raw:
-      "?P\<^sup>t = ((\<not> ok\<^sup><) \<or> Post\<lbrakk>True/ok\<^sup>>\<rbrakk>)"
-    by pred_auto
-  have proj_t: "?P\<^sup>t = ((\<not> ok\<^sup><) \<or> Post)"
-    by (simp only: proj_t_raw assms(3))
+  have f: "(true \<turnstile> Q)\<^sup>f = (\<not> ok\<^sup><)"
+    and t_raw: "(true \<turnstile> Q)\<^sup>t =
+      ((\<not> ok\<^sup><) \<or> Q\<lbrakk>True/ok\<^sup>>\<rbrakk>)"
+    by pred_auto+
   have pre_ok: "((\<not> (\<not> ok\<^sup><)) \<turnstile> T) = (true \<turnstile> T)"
       for T :: "('t, 'e) reactive_angelic_design"
     by pred_auto
-
-  have "AP ?P =
-      RA3AP ((\<not> RA2 (PBMH_ades (\<not> ok\<^sup><))) \<turnstile>
-             RA2 (RA1 (PBMH_ades ((\<not> ok\<^sup><) \<or> Post))))"
-    by (simp only: AP_RA3AP_design comp_apply wf_id proj_f proj_t)
-  also have "... =
-      RA3AP ((\<not> (\<not> ok\<^sup><)) \<turnstile>
-             RA1 ((\<not> ok\<^sup><) \<or> RA2 Post))"
-    by (simp only: PBMH_ades_disj PBMH_ades_not_ok_expr assms(2)
-        RA2_not_ok_expr RA1_RA2_commute'[symmetric] RA2_disj)
-  also have "... = RA3AP (true \<turnstile> RA1 (RA2 Post))"
-    by (simp only: pre_ok design_true_RA1_not_ok)
-  finally show ?thesis
-    by (simp only: RA3AP_design expr_if_idem)
+  show ?thesis
+    by (simp only: AP_RA3AP_design comp_apply rad_wait_false_design
+        rad_wait_false_true assms(1) f t_raw assms(3)
+        PBMH_ades_disj PBMH_ades_not_ok_expr assms(2)
+        RA2_not_ok_expr RA1_RA2_commute'[symmetric] RA2_disj
+        pre_ok design_true_RA1_not_ok RA3AP_design expr_if_idem)
 qed
 
 (* Thesis Lemma L.H.1.5. *)
@@ -240,7 +230,7 @@ lemma AP_wait_false:
        ((P \<^sub>wf)\<^sup>f))) \<turnstile>
      rad_wait_false ((RA2 \<circ> RA1 \<circ> PBMH_ades)
        ((P \<^sub>wf)\<^sup>t)))"
-  by (simp only: AP_design rad_wait_false_design
+  by (simp only: AP_wait_cond_design rad_wait_false_design
       rad_wait_false_wait_cond rad_wait_false_not
       rad_wait_false_idem rad_wait_false_ok_false
       rad_wait_false_ok_true)
@@ -286,10 +276,12 @@ lemma A0_design_absorb:
    A0 ((\<not> X) \<turnstile> Y) = ((\<not> X) \<turnstile> Y)"
   by (simp add: A0_def unrest; pred_auto; blast)
 
-subsubsection \<open>The design body of the AP normal form\<close>
+subsection \<open>Idempotence of AP\<close>
 
 (* The design inside RA3AP in the Theorem 37 normal form is a fixed
-   point of each component healthiness condition of AP. *)
+   point of each component healthiness condition of AP, so RA3AP images
+   of A- and RA2-healthy designs are angelic processes and AP is
+   idempotent. *)
 lemma AP_body_is_H [closure]:
   "((\<not> (RA2 \<circ> PBMH_ades) ((P \<^sub>wf)\<^sup>f)) \<turnstile>
     (RA2 \<circ> RA1 \<circ> PBMH_ades) ((P \<^sub>wf)\<^sup>t)) is \<^bold>H"
@@ -336,56 +328,126 @@ lemma RA3AP_AP_closure [closure]:
   assumes "N is A" "N is RA2"
   shows "RA3AP N is AP"
 proof -
-  have N_H: "N is \<^bold>H"
-    using A_is_H[of N] assms(1) by (simp add: Healthy_def')
   have reform: "((\<not> (N\<^sup>f)) \<turnstile> (N\<^sup>t)) = N"
-  proof -
-    have "((\<not> (N\<^sup>f)) \<turnstile> (N\<^sup>t)) = \<^bold>H N"
-      by (rule sym, rule H1_H2_eq_design)
-    also have "... = N"
-      using N_H by (simp only: Healthy_def')
-    finally show ?thesis .
-  qed
+    using A_is_H[of N] assms(1)
+    by (simp add: Healthy_def' H1_H2_eq_design)
   have "AP (RA3AP N) =
       (RA3AP \<circ> RA2 \<circ> A)
-        ((\<not> ((RA3AP N) \<^sub>wf)\<^sup>f) \<turnstile>
-         ((RA3AP N) \<^sub>wf)\<^sup>t)"
-    by (rule AP_design_form)
-  also have "... =
-      (RA3AP \<circ> RA2 \<circ> A)
         (rad_wait_false ((\<not> (N\<^sup>f)) \<turnstile> (N\<^sup>t)))"
-    by (simp only: rad_wait_false_RA3AP_absorb[simplified comp_apply]
+    by (simp only: AP_design_form
+        rad_wait_false_RA3AP_absorb[simplified comp_apply]
         rad_wait_false_design rad_wait_false_not
         rad_wait_false_ok_false rad_wait_false_ok_true)
-  also have "... = (RA3AP \<circ> RA2 \<circ> A) (rad_wait_false N)"
-    by (simp only: reform)
-  also have "... = (RA3AP \<circ> RA2 \<circ> A) N"
-    by (simp only: comp_apply RA3AP_RA2_A_wait_false_absorb')
   also have "... = RA3AP N"
-    by (simp only: comp_apply Healthy_if[OF assms(1)]
-        Healthy_if[OF assms(2)])
+    by (simp only: reform comp_apply RA3AP_RA2_A_wait_false_absorb'
+        Healthy_if[OF assms(1)] Healthy_if[OF assms(2)])
   finally show ?thesis
     by (rule Healthy_intro)
 qed
 
 lemma AP_idem: "AP (AP P) = AP P"
-proof -
-  let ?N = "((\<not> (RA2 \<circ> PBMH_ades) ((P \<^sub>wf)\<^sup>f)) \<turnstile>
-             (RA2 \<circ> RA1 \<circ> PBMH_ades) ((P \<^sub>wf)\<^sup>t))"
-  have "AP (AP P) = AP (RA3AP ?N)"
-    by (simp only: AP_RA3AP_design)
-  also have "... = RA3AP ?N"
-    by (rule Healthy_if[OF RA3AP_AP_closure[OF
-        AP_body_is_A AP_body_is_RA2]])
-  also have "... = AP P"
-    by (simp only: AP_RA3AP_design)
-  finally show ?thesis .
-qed
+  by (rule Healthy_if, subst AP_RA3AP_design[of P],
+      rule RA3AP_AP_closure, rule AP_body_is_A, rule AP_body_is_RA2)
 
 lemma AP_Idempotent [closure]: "Idempotent AP"
   by (simp add: Idempotent_def AP_idem)
 
 lemma AP_healthy [closure]: "AP P is AP"
   by (simp add: Healthy_def' AP_idem)
+
+subsection \<open>Inherited Healthiness\<close>
+
+lemma AP_PBMH_ades_healthy [closure]: "AP P is PBMH_ades"
+  apply (simp only: AP_RA3AP_design)
+  apply (rule RA3AP_PBMH_ades_closure)
+  apply (rule PBMH_ades_design_closure)
+   apply (simp only: comp_apply,
+      rule RA2_PBMH_ades_closure,
+      rule Healthy_Idempotent[OF PBMH_ades_Idempotent])
+  apply (simp only: comp_apply,
+      rule RA2_PBMH_ades_closure,
+      rule RA1_PBMH_ades_closure,
+      rule Healthy_Idempotent[OF PBMH_ades_Idempotent])
+  done
+
+lemma AP_is_PBMH_ades:
+  assumes "P is AP"
+  shows "P is PBMH_ades"
+  using AP_PBMH_ades_healthy[of P]
+  by (simp only: Healthy_def' Healthy_if[OF assms])
+
+lemma AP_H_healthy [closure]: "AP P is \<^bold>H"
+  by (simp only: AP_wait_cond_design,
+      rule design_is_H1_H2; unrest)
+
+lemma AP_is_H:
+  assumes "P is AP"
+  shows "P is \<^bold>H"
+  using AP_H_healthy[of P]
+  by (simp only: Healthy_def' Healthy_if[OF assms])
+
+lemma AP_wait_false_PBMH_ades:
+  assumes "P is AP"
+  shows "(P \<^sub>wf) is PBMH_ades"
+proof -
+  have P_H: "P is \<^bold>H"
+    by (rule AP_is_H[OF assms])
+  have P_PBMH: "PBMH_ades P = P"
+    using AP_is_PBMH_ades[OF assms]
+    by (simp only: Healthy_def')
+  have P_A1: "A1 P = P"
+    by (simp only: A1_eq_PBMH_ades[OF P_H] P_PBMH)
+  have wf_H: "(P \<^sub>wf) is \<^bold>H"
+    unfolding rad_wait_false_as_state_subst
+    by (rule state_subst_H1_H2_closed[OF P_H])
+  have wf_A1: "A1 (P \<^sub>wf) = (P \<^sub>wf)"
+    using arg_cong[where f=rad_wait_false, OF P_A1]
+    by (simp only: rad_wait_false_as_state_subst A1_state_subst)
+  show ?thesis
+    by (rule Healthy_intro,
+        simp only: A1_eq_PBMH_ades[OF wf_H, symmetric] wf_A1)
+qed
+
+lemma AP_wf_ok_false_PBMH_ades:
+  assumes "P is AP"
+  shows "(P \<^sub>wf)\<^sup>f is PBMH_ades"
+  by (rule Healthy_intro,
+      simp only: PBMH_ades_ok_false
+        Healthy_if[OF AP_wait_false_PBMH_ades[OF assms]])
+
+lemma AP_wf_ok_true_PBMH_ades:
+  assumes "P is AP"
+  shows "(P \<^sub>wf)\<^sup>t is PBMH_ades"
+  by (rule Healthy_intro,
+      simp only: PBMH_ades_ok_true
+        Healthy_if[OF AP_wait_false_PBMH_ades[OF assms]])
+
+abbreviation bottom_AP :: "('t::trace, 'e) reactive_angelic_design"
+    ("\<^bold>\<bottom>\<^sub>A\<^sub>P") where
+"\<^bold>\<bottom>\<^sub>A\<^sub>P \<equiv> AP true"
+
+abbreviation top_AP :: "('t::trace, 'e) reactive_angelic_design"
+    ("\<^bold>\<top>\<^sub>A\<^sub>P") where
+"\<^bold>\<top>\<^sub>A\<^sub>P \<equiv> AP false"
+
+lemma bottom_AP_lower:
+  assumes "P is AP"
+  shows "\<^bold>\<bottom>\<^sub>A\<^sub>P \<sqsubseteq> P"
+proof -
+  have "AP true \<sqsubseteq> AP P"
+    by (rule AP_mono; pred_auto)
+  then show ?thesis
+    by (simp only: Healthy_if[OF assms])
+qed
+
+lemma top_AP_upper:
+  assumes "P is AP"
+  shows "P \<sqsubseteq> \<^bold>\<top>\<^sub>A\<^sub>P"
+proof -
+  have "AP P \<sqsubseteq> AP false"
+    by (rule AP_mono; pred_auto)
+  then show ?thesis
+    by (simp only: Healthy_if[OF assms])
+qed
 
 end
