Angelic_CSP.thy
@@ -1,6 +1,6 @@
 section \<open>Angelic CSP via UTP\<close>
 
 theory Angelic_CSP
-  imports utp_ap_nd
+  imports utp_ap_nd utp_ap_examples
 begin
 end
