utp_ap_examples.thy
@@ -1,0 +1,48 @@
+section \<open>Angelic Process Examples\<close>
+
+text \<open>
+  The worked examples of the paper's Section 7, collected apart from
+  the healthiness, correspondence, and operator theories.
+\<close>
+
+theory utp_ap_examples
+  imports utp_ap_rad
+begin
+
+(* Paper Example 22: Theorem 39 applied to Chaos_RAD = RAD true. *)
+lemma H1_Chaos_RAD_example:
+  "H1 (Chaos\<^sub>R\<^sub>A\<^sub>D :: ('t::trace, 'e) reactive_angelic_design) =
+   ((($rad_wait_lens\<^sup><)\<^sub>e \<or> (\<not> RA1 true)) \<turnstile>
+     (($rad_wait_lens\<^sup><)\<^sub>e \<and> ades_state_choice))"
+  by (simp only: Chaos_RAD_RAD H1_RAD_design[simplified comp_apply]
+      rad_wait_false_true subst_pred(1) PBMH_ades_true RA2_true
+      RA2_RA1_true RA3AP_design_post;
+      pred_auto add: rad_trace_extensions_def)
+
+(* Paper Example 23. *)
+lemma H1_Skip_RAD_example:
+  "H1 (Skip\<^sub>R\<^sub>A\<^sub>D :: ('t::trace, 'e) reactive_angelic_design) =
+   (true \<turnstile> RA3AP skip_post)"
+  by (simp only: Skip_RAD_def comp_apply
+      H1_RA_A_true_design[where P=skip_post,
+        simplified rad_wait_false_skip_post skip_post_ok_out_subst comp_apply]
+      skip_post_PBMH RA1_skip_post RA2_skip_post)
+
+(* Paper Example 24 *)
+lemma RA1_H1_Chaos_RAD_example:
+  "RA1 ((($rad_wait_lens\<^sup><)\<^sub>e \<or> (\<not> RA1 true)) \<turnstile>
+      (($rad_wait_lens\<^sup><)\<^sub>e \<and> ades_state_choice)) =
+   (Chaos\<^sub>R\<^sub>A\<^sub>D :: ('t::trace, 'e) reactive_angelic_design)"
+  by (simp only: H1_Chaos_RAD_example[symmetric] Chaos_RAD_RAD
+      RA1_H1_RAD[simplified comp_apply])
+
+(* Paper Example 25: H1 after mapping the bottom AP through RA1. *)
+lemma H1_RA1_bottom_AP_example:
+  "(H1 \<circ> RA1) (\<^bold>\<bottom>\<^sub>A\<^sub>P ::
+      ('t::trace, 'e) reactive_angelic_design) =
+   ((($rad_wait_lens\<^sup><)\<^sub>e \<or> (\<not> RA1 true)) \<turnstile>
+    (($rad_wait_lens\<^sup><)\<^sub>e \<and> ades_state_choice))"
+  by (simp only: comp_apply RA1_AP_RAD[simplified comp_apply]
+      bottom_RAD_is_Chaos H1_Chaos_RAD_example)
+
+end
